mm_map_root proof with all sub-lemmas factored out and put in the correct files

coq-verification/src/Concrete/StateProofs.v
@@ -56,17 +56,58 @@ Section Proofs.
            end.
   Qed.
 
-  (* given a sequence of page table indices, says whether the address is found
-     under the same sequence of page table indexing *)
-  Definition is_under_path (indices : list nat) (addr : uintpaddr_t) : bool :=
-    forallb
-      (fun '(lvl, i) => get_index lvl addr =? i)
-      (combine (seq 0 4) indices).
+  Definition all_root_ptables : list mm_ptable :=
+    hafnium_ptable :: map vm_ptable vms.
+
+  Definition all_root_ptable_pointers : list ptable_pointer :=
+    hafnium_root_tables ++ flat_map vm_root_tables vms.
+
+  Fixpoint pointer_in_table'
+             (deref : ptable_pointer -> mm_page_table) (ptr : ptable_pointer)
+             (t : mm_page_table) (lvls_to_go : nat) : Prop :=
+    match lvls_to_go with
+    | 0 => False
+    | S lvls_to_go' =>
+      let lvl := 4 - lvls_to_go in
+      Exists
+        (fun i =>
+           match get_entry t i with
+           | Some pte =>
+             if arch_mm_pte_is_table pte lvl
+             then 
+               let next_t_ptr :=
+                   ptable_pointer_from_address (arch_mm_table_from_pte pte lvl) in
+               if ptable_pointer_eq_dec ptr next_t_ptr
+               then True
+               else pointer_in_table' deref ptr (deref next_t_ptr) lvls_to_go'
+             else False
+           | None => False
+           end)
+        (seq 0 MM_PTE_PER_PAGE)
+    end.
+
+  Definition pointer_in_table
+             (deref : ptable_pointer -> mm_page_table) (ptr : ptable_pointer)
+             (t : mm_page_table) : Prop :=
+    Forall (pointer_in_table' deref ptr t) (seq 0 4).
+
+  Definition deref_noncircular (c : concrete_state) : Prop :=
+    forall ptr,
+      ~ pointer_in_table c.(ptable_deref) ptr (c.(ptable_deref) ptr).
+
+  (* TODO : It's not clear that this definition is the correct approach. Consider
+     other ways to keep track of the fact that page tables don't have circular
+     references and don't use any locations in the freelist. *)
+  Definition pointers_ok (c : concrete_state) (ppool : mpool) : Prop :=
+    deref_noncircular c
+    /\ (forall ptr,
+           mpool_contains ppool ptr <->
+           (forall ptr2, ~ pointer_in_table c.(ptable_deref) ptr (c.(ptable_deref) ptr2))).
 
   (* We haven't formalized anywhere that pointers don't repeat, so we return a
      list of all locations where the provided pointer exists even though we
      expect there is only one. *)
-  Fixpoint index_sequences_to_pointer' (ptable_deref : ptable_pointer -> mm_page_table)
+  Fixpoint index_sequences_to_pointer'' (ptable_deref : ptable_pointer -> mm_page_table)
            (ptr : ptable_pointer) (root : ptable_pointer) (lvls_to_go : nat)
     : list (list nat) :=
     match lvls_to_go with
@@ -88,21 +129,30 @@ Section Proofs.
                        (arch_mm_table_from_pte pte lvl) in
                  map
                    (cons index)
-                   (index_sequences_to_pointer'
+                   (index_sequences_to_pointer''
                       ptable_deref ptr next_root lvls_to_go')
                else nil
              | None => nil
              end)
           (seq 0 MM_PTE_PER_PAGE)
     end.
+  Fixpoint index_sequences_to_pointer'
+           (ptable_deref : ptable_pointer -> mm_page_table)
+           (ptr : ptable_pointer) (root_index : nat)
+           (root_ptrs : list ptable_pointer) : list (list nat) :=
+    match root_ptrs with
+    | nil => nil
+    | cons root_ptr root_ptrs' =>
+      (map (cons root_index)
+           (index_sequences_to_pointer'' ptable_deref ptr root_ptr 4))
+        ++
+        index_sequences_to_pointer' ptable_deref ptr (S root_index) root_ptrs'
+    end.
   Definition index_sequences_to_pointer
-             (ptable_deref : ptable_pointer -> mm_page_table)
-             (ptr : ptable_pointer) (root : ptable_pointer) : list (list nat) :=
-    index_sequences_to_pointer' ptable_deref ptr root 4.
-
-  (* TODO : move *)
-  Axiom va_init : uintvaddr_t -> vaddr_t.
-  Axiom pa_from_va : vaddr_t -> paddr_t.
+           (ptable_deref : ptable_pointer -> mm_page_table)
+           (ptr : ptable_pointer) (root_ptable : mm_ptable) :=
+    index_sequences_to_pointer'
+      ptable_deref ptr 0 (ptr_from_va (va_from_pa root_ptable.(root))).
 
   Definition abstract_change_attrs (abst : abstract_state)
              (a : paddr_t) (e : entity_id) (owned valid : bool) :=
@@ -126,23 +176,34 @@ Section Proofs.
            else prev)
     |}.
 
+  (* given a sequence of page table indices, says whether the address is found
+     under the same sequence of page table indexing *)
+  Definition is_under_path (indices : list nat) (addr : uintpaddr_t) : bool :=
+    forallb
+      (fun '(lvl, i) => get_index lvl addr =? i)
+      (combine (seq 0 4) indices).
+
+  Definition addresses_under_pointer_in_range
+             (deref : ptable_pointer -> mm_page_table)
+             (ptr : ptable_pointer) (root_ptable : mm_ptable)
+             (begin end_ : uintvaddr_t) : list paddr_t :=
+    let vrange := map N.of_nat (seq (N.to_nat begin) (N.to_nat end_)) in
+    let prange := map (fun va => pa_from_va (va_init va)) vrange in
+    let paths := index_sequences_to_pointer deref ptr root_ptable in
+    filter
+      (fun a => existsb (fun p => is_under_path p (pa_addr a)) paths) prange.
+
   Definition abstract_reassign_pointer_for_entity
              (abst : abstract_state) (conc : concrete_state)
              (ptr : ptable_pointer) (owned valid : bool)
-             (e : entity_id) (root_ptable : ptable_pointer)
+             (e : entity_id) (root_ptable : mm_ptable)
              (begin end_ : uintvaddr_t) : abstract_state :=
-    let vrange := map N.of_nat (seq (N.to_nat begin) (N.to_nat end_)) in
-    let prange := map (fun va => pa_from_va (va_init va)) vrange in
-    let paths := index_sequences_to_pointer
-                   conc.(ptable_deref) ptr root_ptable in
-    let under_pointer : uintpaddr_t -> bool :=
-        fun addr =>
-          existsb (fun p => is_under_path p addr) paths in
     fold_right
       (fun pa abst =>
          abstract_change_attrs abst pa e owned valid)
       abst
-      (filter (fun pa => under_pointer (pa_addr pa)) prange).
+      (addresses_under_pointer_in_range
+         conc.(ptable_deref) ptr root_ptable begin end_).
 
   (* Update the abstract state to make everything under the given pointer have
      the provided new owned/valid bits. *)
@@ -161,14 +222,13 @@ Section Proofs.
     (* update the state with regard to Hafnium *)
     let abst :=
         abstract_reassign_pointer_for_entity
-          abst conc ptr s1_owned s1_valid (inr hid) hafnium_root_ptable
-          begin end_ in
+          abst conc ptr s1_owned s1_valid (inr hid) hafnium_ptable begin end_ in
 
     (* update the state with regard to each VM *)
     fold_right
       (fun (v : vm) (abst : abstract_state) =>
          abstract_reassign_pointer_for_entity
-           abst conc ptr s2_owned s2_valid (inl v.(vm_id)) (vm_root_ptable v)
+           abst conc ptr s2_owned s2_valid (inl v.(vm_id)) (vm_ptable v)
            begin end_)
       abst
       vms.
@@ -197,12 +257,104 @@ Section Proofs.
     cbv [vm_page_valid haf_page_valid vm_page_owned haf_page_owned].
     cbn [ptable_deref].
     basics; try solver.
-    (* 4 subgoals *)
+    (* TODO: 4 subgoals *)
   Admitted.
 
   Lemma abstract_reassign_pointer_trivial abst conc ptr attrs i :
     abstract_state_equiv (abstract_reassign_pointer abst conc ptr attrs i i)
                          abst.
+  Admitted. (* TODO *)
+
+  Lemma abstract_reassign_pointer_for_entity_change_concrete
+        abst conc conc' ptr owned valid e root_ptr begin end_ :
+    index_sequences_to_pointer conc.(ptable_deref) ptr root_ptr
+    = index_sequences_to_pointer conc'.(ptable_deref) ptr root_ptr ->
+    abstract_reassign_pointer_for_entity
+      abst conc ptr owned valid e root_ptr begin end_
+    = abstract_reassign_pointer_for_entity
+        abst conc' ptr owned valid e root_ptr begin end_.
+  Proof.
+    cbv beta iota delta [abstract_reassign_pointer_for_entity
+                           addresses_under_pointer_in_range].
+    intro Heq. rewrite Heq. reflexivity.
+  Qed.
+
+  Lemma abstract_reassign_pointer_change_concrete
+        abst conc conc' ptr attrs begin_index end_index :
+    Forall (fun root =>
+              index_sequences_to_pointer conc.(ptable_deref) ptr root
+              = index_sequences_to_pointer conc'.(ptable_deref) ptr root)
+           all_root_ptables ->
+    abstract_reassign_pointer abst conc ptr attrs begin_index end_index
+    = abstract_reassign_pointer abst conc' ptr attrs begin_index end_index.
+  Proof.
+    cbv [abstract_reassign_pointer all_root_ptables].
+    repeat match goal with
+           | _ => progress basics
+           | _ => progress invert_list_properties
+           | H : _ |- _ => apply Forall_map in H; rewrite Forall_forall in H
+           | _ =>
+             rewrite abstract_reassign_pointer_for_entity_change_concrete
+               with (conc':=conc') by eauto
+           | _ => apply fold_right_ext
+           | _ => solve
+                    [auto using
+                          abstract_reassign_pointer_for_entity_change_concrete]
+           end.
+  Qed.
+
+  (* has_uniform_attrs doesn't care if we reassign the pointer we started from *)
+  (* TODO : fill in preconditions *)
+  Lemma has_uniform_attrs_reassign_pointer c ptr new_table t level attrs begin end_:
+    ~ pointer_in_table (ptable_deref c) ptr t ->
+    has_uniform_attrs (ptable_deref c) t level attrs begin end_ ->
+    has_uniform_attrs
+      (ptable_deref (reassign_pointer c ptr new_table))
+      t level attrs begin end_.
+  Admitted. (* TODO *)
+
+  Definition no_addresses_in_range deref ptr begin end_ : Prop :=
+    Forall
+      (fun root_ptable =>
+         addresses_under_pointer_in_range deref ptr root_ptable begin end_ = nil)
+      all_root_ptables.
+
+  (* abstract_reassign_pointer is a no-op if the given tables don't have any
+     addresses in range *)
+  (* TODO: fill in preconditions; likely needs to know that the table is at the
+     right level *)
+  Lemma abstract_reassign_pointer_low
+        abst conc attrs begin end_ t_ptrs :
+    Forall
+      (fun ptr => no_addresses_in_range conc.(ptable_deref) ptr begin end_)
+      t_ptrs ->
+    abstract_state_equiv
+      abst
+      (fold_left
+         (fun abst t_ptr =>
+            abstract_reassign_pointer abst conc t_ptr attrs begin end_)
+         t_ptrs
+         abst).
   Admitted.
 
+  (* we can expand the range to include pointers that are out of range *)
+  (* TODO: fill in preconditions; likely needs to know that the table is at the
+     right level *)
+  Lemma abstract_reassign_pointer_high
+        abst conc attrs begin end_ i t_ptrs :
+    Forall
+      (fun ptr => no_addresses_in_range conc.(ptable_deref) ptr begin end_)
+      (skipn i t_ptrs) ->
+    abstract_state_equiv
+      (fold_left
+         (fun abst t_ptr =>
+            abstract_reassign_pointer abst conc t_ptr attrs begin end_)
+         (firstn i t_ptrs)
+         abst)
+      (fold_left
+         (fun abst t_ptr =>
+            abstract_reassign_pointer abst conc t_ptr attrs begin end_)
+         t_ptrs
+         abst).
+  Admitted.
 End Proofs.
