coq-verification/src/Util/BinNat.v
@@ -1,6 +1,7 @@
 Require Import Coq.Arith.PeanoNat.
 Require Import Coq.NArith.BinNat.
 Require Import Coq.NArith.Nnat.
+Require Import Hafnium.Util.Tactics.
 Local Open Scope N_scope.
 
 Module N.
@@ -18,4 +19,28 @@ Module N.
     rewrite <-N.compare_le_iff, <-Nat.compare_le_iff.
     rewrite N2Nat.inj_compare. reflexivity.
   Qed.
+
+  Lemma to_nat_lt_iff x y : (N.to_nat x < N.to_nat y)%nat <-> x < y.
+  Admitted. (* TODO *)
+
+  (* TODO: move *)
+  Lemma div2_lnot a n : N.div2 (N.lnot a n) = N.lnot (N.div2 a) (N.pred n).
+  Admitted. (* TODO *)
+    
+  Lemma lnot_shiftr a n m :
+    N.shiftr (N.lnot a n) m = N.lnot (N.shiftr a m) (n - m).
+  Proof.
+    rewrite <-(Nnat.N2Nat.id m).
+    induction (N.to_nat m).
+    { rewrite !N.shiftr_0_r.
+      rewrite N.sub_0_r. reflexivity. }
+    { rewrite Nnat.Nat2N.inj_succ.
+      rewrite !N.shiftr_succ_r.
+      rewrite N.sub_succ_r.
+      rewrite <-div2_lnot.
+      solver. }
+  Qed.
+
+  Lemma log2_add_shiftl_1 a b : b <= N.log2 (a + (N.shiftl 1 b)).
+  Admitted. (* TODO *)
 End N.
